Iris/Iris/ProgramLogic/EctxLanguage.lean
@@ -1,0 +1,368 @@
+module
+
+meta import Iris.Std.RocqPorting
+public import Iris.ProgramLogic.Language
+
+namespace Iris.ProgramLogic
+
+@[expose] public section
+
+variable {Expr : Type e}{Val : Type v}{State : Type σ}{Obs : Type o}
+variable {Ectx : Type c}
+
+class IsEvContext (Ectx : Type c) where
+  empty : Ectx
+  comp  : Ectx → Ectx → Ectx
+export IsEvContext (empty comp)
+
+class EvContext (Expr : Type e) (Ectx : outParam <| Type c)
+  extends IsEvContext Ectx
+  where
+  fill  : Ectx → Expr → Expr
+  fill_empty (e : Expr) : fill empty e = e
+  fill_comp K₁ K₂ (e : Expr) :
+    fill K₁ (fill K₂ e) = fill (comp K₁ K₂) e
+  fill_inj {K} : Function.Injective (fill K)
+export EvContext (fill)
+
+attribute [grind =] EvContext.fill_empty
+attribute [grind =_] EvContext.fill_comp
+
+attribute [local simp] EvContext.fill_inj Function.Injective.eq_iff
+
+class BaseStep
+    (Expr : Type e)
+    (State : outParam (Type σ))
+    (Obs : outParam (Type o)) where
+  /-- The base reduction relation of the language -/
+  baseStep : Expr × State → List Obs → Expr × State × List Expr → Prop
+
+namespace BaseStep
+
+variable [BaseStep Expr State Obs]
+
+@[inherit_doc BaseStep.baseStep]
+scoped notation conf:40 " -<" obs:max ">->ᵇ " conf':41  => BaseStep.baseStep conf obs conf'
+
+@[grind]
+inductive ToPrimStep [EvContext Expr Ectx] [BaseStep Expr State Obs]
+  (obs : List Obs) (eₜ : List Expr) (σ₁ σ₂ : State) :
+    Expr → Expr → Prop where
+  | intro : ∀ (e₁ e₂) (K : Ectx),
+    (e₁, σ₁) -<obs>->ᵇ (e₂,σ₂,eₜ) →
+    ToPrimStep obs eₜ σ₁ σ₂ (fill K e₁) (fill K e₂)
+
+@[match_pattern]
+abbrev ToPrimStep.ofBaseStep [EvContext Expr Ectx] [BaseStep Expr State Obs]
+  {e₁ : Expr} {σ₁ obs e₂ σ₂ eₜ} (K : Ectx) :
+    (e₁, σ₁) -<obs>->ᵇ (e₂,σ₂,eₜ) →
+    ToPrimStep obs eₜ σ₁ σ₂ (fill K e₁) (fill K e₂) :=
+  (ToPrimStep.intro _ _ _ ·)
+
+@[match_pattern]
+abbrev ToPrimStep.ofBaseStep' [EvContext Expr Ectx] [BaseStep Expr State Obs]
+  {e e' e₁ : Expr} {σ₁ obs e₂ σ₂ eₜ} (K : Ectx) :
+    fill K e₁ = e →
+    fill K e₂ = e' →
+    (e₁, σ₁) -<obs>->ᵇ (e₂,σ₂,eₜ) →
+    ToPrimStep obs eₜ σ₁ σ₂ e e' := fun
+  | rfl, rfl => (ToPrimStep.intro _ _ _ ·)
+
+@[grind]
+instance [BaseStep Expr State Obs] [EvContext Expr Ectx] :
+    PrimStep Expr State (List Obs) where
+  primStep
+  | (e₁, σ₁), obs, (e₂, σ₂, eₜ) =>
+    ToPrimStep obs eₜ σ₁ σ₂ e₁ e₂
+
+@[rocq_alias base_reducible]
+def reducible : Expr × State → Prop
+| (e,σ) => ∃ obs e' σ' eₜ, (e,σ) -<obs>->ᵇ (e',σ',eₜ)
+
+@[rocq_alias base_reducible_no_obs]
+def reducibleNoObs : Expr × State → Prop
+| (e,σ) => ∃ e' σ' eₜ, (e,σ) -<[]>->ᵇ (e',σ', eₜ)
+
+@[rocq_alias base_irreducible]
+def irreducible : Expr × State → Prop
+| (e,σ) => ∀ obs e' σ' eₜ, ¬ (e,σ) -<obs>->ᵇ (e',σ',eₜ)
+
+@[rocq_alias base_stuck]
+def stuck [ToVal Expr Val]: Expr × State → Prop
+| (e,σ) => toVal e = none ∧ irreducible (e,σ)
+
+variable {e : Expr}{σ : State}
+
+@[rocq_alias not_base_reducible, grind =]
+theorem not_reducible_iff_irreducible :
+    (¬ reducible (e, σ)) ↔ irreducible (e, σ) := by
+  grind only [reducible, irreducible]
+
+@[rocq_alias base_reducible_no_obs_reducible, grind .]
+theorem reducible_of_reducibleNoObs :
+    reducibleNoObs (e, σ) → reducible (e, σ) := by
+  grind only [reducibleNoObs, reducible]
+
+end BaseStep
+
+open BaseStep in
+class EctxLanguage
+    (Expr  : Type e)
+    (Ectx  : outParam <| Type c)
+    (State : outParam <| Type σ)
+    (Obs   : outParam <| Type o)
+    (Val   : outParam <| Type v)
+  extends
+    BaseStep Expr State Obs,
+    ToVal Expr Val,
+    EvContext Expr Ectx where
+  fill_val K e :
+    (toVal (fill K e)).isSome →
+    (toVal e).isSome
+  step_by_val {K' K_redex e₁' e₁_redex σ₁ obs e₂ σ₂ eₜ } :
+    fill K' e₁' = fill K_redex e₁_redex →
+    toVal e₁' = none →
+    (e₁_redex, σ₁) -<obs>->ᵇ (e₂, σ₂, eₜ) →
+    ∃ K'', K_redex = comp K' K''
+
+  val_stuck : ∀ {e} {σ : State} {obs e' σ' eₜ},
+    (e, σ) -<obs>->ᵇ (e', σ', eₜ) → toVal e = none
+
+  /- NOTE: Steps now occur only in redex posiitons! -/
+  base_ctx_step_val {K e σ₁ obs e₂ σ₂ eₜ} :
+    (fill K e, σ₁) -<obs>->ᵇ (e₂, σ₂, eₜ) →
+    (toVal e).isSome ∨ K = empty
+
+attribute [grind .] EctxLanguage.val_stuck
+
+namespace EctxLanguage
+open BaseStep
+
+variable [EctxLanguage Expr Ectx State Obs Val]
+
+@[grind =>]
+theorem fill_not_val K (e : Expr) :
+    (toVal e) = none → (toVal (fill K e)) = none := by
+  grind only [!fill_val, Option.not_isSome_iff_eq_none]
+
+
+@[rocq_alias subredexes_are_values]
+def subredexesAreValues (e : Expr) := ∀ (K : Ectx) e',
+  e = fill K e' →
+  toVal e' = none →
+  K = empty
+
+@[rocq_alias LanguageOfEctx]
+instance : Language Expr State Obs Val where
+  val_stuck {e σ obs e' σ' eₜ} primStep := by
+    rcases primStep with ⟨K, bstep⟩
+    grind only [val_stuck, fill_not_val]
+
+@[rocq_alias base_atomic]
+def baseAtomic (a : Language.Atomicity) (e : Expr) : Prop :=
+    ∀ σ obs e' σ' eₜ,
+      (e,σ) -<obs>->ᵇ (e',σ',eₜ) →
+      match a with
+      | .WeaklyAtomic => PrimStep.irreducible (e',σ')
+      | .StronglyAtomic => (toVal e').isSome
+
+variable {e e' e₁ e₂ : Expr} {σ σ' σ₁ σ₂ : State}
+variable {K K' K₁ K₂ : Ectx} {obs obs' : List Obs}
+variable {eₜ eₜ : List Expr}
+
+open EvContext in
+@[rocq_alias base_redex_unique]
+theorem base_redex_unique K K' (e e' : Expr) σ σ' :
+    fill K e = fill K' e' →
+    reducible (e, σ) →
+    reducible (e', σ') →
+    K = comp K' empty ∧
+    e = e' := by
+  rintro heq ⟨obs, e₂, σ₂, eₜ, bstep⟩ ⟨obs', e₂', σ₂', eₜ', bstep'⟩
+  obtain ⟨K'', rfl⟩ := step_by_val heq.symm (by grind) bstep
+  simp only [← fill_comp, fill_inj, Function.Injective.eq_iff] at heq
+  subst heq
+  match base_ctx_step_val bstep' with
+  | .inl h =>
+    grind only [val_stuck, = Option.isSome_none]
+  | .inr h =>
+    grind only [fill_empty]
+
+open PrimStep in
+@[rocq_alias base_prim_step]
+theorem primStep_of_baseStep {e₁ : Expr}{σ₁ obs e₂ σ₂ eₜ}:
+    (e₁, σ₁) -<obs>->ᵇ (e₂, σ₂, eₜ) →
+    (e₁, σ₁) -<obs>-> (e₂, σ₂, eₜ) := by
+  intros h
+  have := ToPrimStep.ofBaseStep empty h
+  simpa only [EvContext.fill_empty]
+
+open PrimStep in
+theorem baseStep_of_primStep {e₁ : Expr}{σ₁ obs e₂ σ₂ eₜ}:
+    (e₁, σ₁) -<obs>-> (e₂, σ₂, eₜ) →
+    subredexesAreValues e₁ →
+    (e₁, σ₁) -<obs>->ᵇ  (e₂, σ₂, eₜ) := fun pstep subredexValues =>
+  have ⟨e₁, e₂, K, bstep⟩ := pstep
+  have K_empty := subredexValues K e₁ rfl (val_stuck bstep)
+  by grind only [EvContext.fill_empty]
+
+open PrimStep in
+@[grind =>]
+theorem baseStep_iff_primStep_of_subredexesAreValues {e₁ : Expr}{σ₁ obs e₂ σ₂ eₜ}:
+    subredexesAreValues e₁ →
+    ((e₁, σ₁) -<obs>-> (e₂, σ₂, eₜ) ↔
+    (e₁, σ₁) -<obs>->ᵇ  (e₂, σ₂, eₜ)) := fun subredexValues =>
+  ⟨(baseStep_of_primStep · subredexValues), primStep_of_baseStep⟩
+
+@[rocq_alias base_step_not_stuck]
+theorem base_step_not_stuck {e : Expr} {σ obs e' σ' eₜ} :
+    (e, σ) -<obs>->ᵇ (e', σ', eₜ) → PrimStep.notStuck (e, σ) :=
+  Language.notStuck_of_primStep ∘ primStep_of_baseStep
+
+open PrimStep in
+@[rocq_alias fill_prim_step]
+theorem fill_primStep (K : Ectx) {e : Expr} {σ obs e' σ' eₜ} :
+    (e, σ) -<obs>-> (e', σ', eₜ) →
+    (fill K e, σ) -<obs>-> (fill K e', σ', eₜ) := fun ⟨e₁, e₂, K₁, pstep⟩ => by
+    have := ToPrimStep.ofBaseStep (comp K K₁) pstep
+    simpa only [EvContext.fill_comp]
+
+@[rocq_alias fill_reducible]
+theorem fill_reducible (K : Ectx) {e : Expr} {σ} :
+    PrimStep.reducible (e, σ) → PrimStep.reducible (fill K e, σ) :=
+  fun ⟨obs, e', σ', eₜ, h⟩ =>
+    ⟨obs, fill K e', σ', eₜ, fill_primStep K h⟩
+
+@[rocq_alias fill_reducible_no_obs]
+theorem reducibleNoObs_fill (K : Ectx) {e : Expr} {σ : State} :
+    PrimStep.reducibleNoObs (e, σ) →
+    PrimStep.reducibleNoObs (fill K e, σ) :=
+  fun ⟨e', σ', eₜ, h⟩ =>
+    ⟨fill K e', σ', eₜ, fill_primStep K h⟩
+
+@[rocq_alias base_prim_reducible]
+theorem primStep_reducible_of_baseStep_reducible :
+    BaseStep.reducible (e, σ) →
+    PrimStep.reducible (e, σ) := fun ⟨obs, e', σ', eₜ, bstep⟩ =>
+  ⟨obs, e', σ', eₜ, primStep_of_baseStep bstep⟩
+
+@[rocq_alias base_prim_fill_reducible]
+theorem primStep_reducible_fill_of_baseStep_reducible :
+    BaseStep.reducible (e, σ) →
+    PrimStep.reducible (fill K e, σ) := fun ⟨obs, e', σ', eₜ, bstep⟩ =>
+  ⟨obs, fill K e', σ', eₜ, .ofBaseStep K bstep⟩
+
+@[rocq_alias base_prim_reducible_no_obs]
+theorem primStep_reducibleNoObs_of_baseStep_reducibleNoObs :
+    BaseStep.reducibleNoObs (e, σ) →
+    PrimStep.reducibleNoObs (e, σ) := fun ⟨e', σ', eₜ, bstep⟩ =>
+  ⟨e', σ', eₜ, primStep_of_baseStep bstep⟩
+
+@[rocq_alias base_prim_fill_reducible_no_obs]
+theorem primStep_reducibleNoObs_fill_of_baseStep_reducibleNoObs :
+    BaseStep.reducibleNoObs (e, σ) →
+    PrimStep.reducibleNoObs (fill K e, σ) := fun ⟨e', σ', eₜ, bstep⟩ =>
+  ⟨fill K e', σ', eₜ, .ofBaseStep K bstep⟩
+
+@[rocq_alias base_prim_irreducible]
+theorem baseStep_irreducible_of_primStep_irreducible :
+    PrimStep.irreducible (e, σ) →
+    BaseStep.irreducible (e, σ) := fun h obs e' σ' eₜ bstep =>
+  h obs e' σ' eₜ <| primStep_of_baseStep bstep
+
+@[rocq_alias prim_base_reducible]
+theorem baseStep_reducible_of_primStep_reducible :
+    PrimStep.reducible (e, σ) →
+    subredexesAreValues e →
+    BaseStep.reducible (e, σ) := fun ⟨obs, e', σ', eₜ, pstep⟩ subredexValues =>
+  ⟨obs, e', σ', eₜ, baseStep_of_primStep pstep subredexValues⟩
+
+@[rocq_alias prim_base_irreducible]
+theorem primStep_irreducible_of_baseStep_irreducible :
+    BaseStep.irreducible (e, σ) →
+    subredexesAreValues e →
+    PrimStep.irreducible (e, σ) := fun birred subredexValues obs e' σ' eₜ pstep =>
+  birred obs e' σ' eₜ (baseStep_of_primStep pstep subredexValues)
+
+@[rocq_alias base_stuck_stuck]
+theorem primStep_stuck_of_baseStep_stuck :
+    BaseStep.stuck (e, σ) →
+    subredexesAreValues e →
+    PrimStep.stuck (e, σ) := fun ⟨toVal_none, birred⟩ subredexValues =>
+  ⟨toVal_none, primStep_irreducible_of_baseStep_irreducible birred subredexValues⟩
+
+@[rocq_alias ectx_language_atomic, implicit_reducible]
+def Atomic.ofBaseAtomic (a : Language.Atomicity) :
+    baseAtomic a e →
+    subredexesAreValues e →
+    Language.Atomic a e := fun batomic subredexValues => {
+      atomic := fun σ obs e' σ' eₜ pstep =>
+        by grind [baseAtomic]
+    }
+
+open PrimStep in
+@[rocq_alias base_reducible_prim_step_ctx]
+theorem exists_baseStep_of_primStep_fill_of_redex_baseStep_reducible :
+    BaseStep.reducible (e₁, σ₁) →
+    (fill K e₁, σ₁) -<obs>-> (e', σ₂, eₜ) →
+    ∃ e₂, e' = fill K e₂ ∧ (e₁, σ₁) -<obs>->ᵇ (e₂, σ₂, eₜ) := by
+  generalize heq : fill K e₁ = e at *
+  rintro ⟨obs', e₂, σ₂', eₜ', bstep⟩ ⟨e₁', e₂', K, bstep'⟩
+  obtain ⟨K'', rfl⟩ := step_by_val heq (by grind) bstep'
+  simp only [← EvContext.fill_comp, EvContext.fill_inj, Function.Injective.eq_iff] at heq ⊢
+  subst heq
+  have : K'' = empty := by grind only [val_stuck, = Option.isSome_none, base_ctx_step_val bstep]
+  grind only [= EvContext.fill_empty]
+
+open PrimStep in
+@[rocq_alias base_reducible_prim_step]
+theorem baseStep_of_primStep_of_baseStep_reducible :
+    BaseStep.reducible (e₁, σ₁) →
+    (e₁, σ₁) -<obs>-> (e₂, σ₂, eₜ) →
+    (e₁, σ₁) -<obs>->ᵇ (e₂, σ₂, eₜ) := fun bred pstep =>
+  have ⟨e₂', heq, bstep⟩ := exists_baseStep_of_primStep_fill_of_redex_baseStep_reducible (K := empty) bred (EvContext.fill_empty e₁ ▸ pstep)
+  heq ▸ (EvContext.fill_empty e₂' |>.symm ▸ bstep)
+
+open PrimStep in
+instance (K : Ectx) : Language.Context (fill (Expr := Expr) K) where
+  toVal_eq_none_fill := fill_not_val K _
+  primStep_fill {e σ obs e' σ' eₜ} := fun ⟨e₁, e₂, K', bstep⟩ =>
+    EvContext.fill_comp K K' e₁ ▸
+    EvContext.fill_comp K K' e₂ ▸
+    .ofBaseStep (comp K K') bstep
+  primStep_fill_inv {e σ obs K_e' σ' eₜ} toVal_none pstep := by
+    generalize heq : fill K e = K_e at *
+    have ⟨e₁, e₂, K', bstep⟩ := pstep
+    obtain ⟨K'', rfl⟩:= step_by_val heq toVal_none bstep
+    simp only [← EvContext.fill_comp, EvContext.fill_inj, Function.Injective.eq_iff,
+      exists_eq_left'] at *
+    subst heq
+    exact ToPrimStep.ofBaseStep K'' bstep
+
+@[rocq_alias pure_base_step]
+structure PureBaseStep (e₁ e₂ : Expr) : Prop where
+  safe : ∀ σ : State, BaseStep.reducibleNoObs (e₁, σ)
+  deterministic : ∀ {σ₁ σ₂ : State} {obs e₂' eₜ},
+    (e₁, σ₁) -<obs>->ᵇ (e₂', σ₂, eₜ) →
+    obs = [] ∧ σ₁ = σ₂ ∧ e₂ = e₂' ∧ eₜ = []
+
+@[inherit_doc BaseStep.baseStep]
+scoped notation conf:40 " -ᵖ->ᵇ " conf':41  => PureBaseStep conf conf'
+
+open Language in
+@[rocq_alias pure_base_step_pure_step]
+theorem purePrimStep_of_pureBaseStep :
+    e₁ -ᵖ->ᵇ e₂ →
+    e₁ -ᵖ-> e₂ := fun ⟨bsafe, bdet⟩ =>
+  have psafe := (primStep_reducibleNoObs_of_baseStep_reducibleNoObs <| bsafe ·)
+  have bred := (BaseStep.reducible_of_reducibleNoObs <| bsafe ·)
+  ⟨ psafe , fun pstep => bdet <| baseStep_of_primStep_of_baseStep_reducible (bred _) pstep⟩
+
+open Language in
+@[rocq_alias pure_exec_fill]
+theorem pureExec_fill φ n :
+    PureExec φ n e₁ e₂ →
+    PureExec φ n (fill K e₁) (fill K e₂) :=
+  Language.pureExec_fill _
+
+end EctxLanguage
