Iris/Iris/ProgramLogic/EctxiLanguage.lean
@@ -1,0 +1,181 @@
+module
+
+meta import Iris.Std.RocqPorting
+public import Iris.ProgramLogic.Language
+public import Iris.ProgramLogic.EctxLanguage
+
+namespace Iris.ProgramLogic
+
+@[expose] public section
+
+variable {Expr : Type e}{Val : Type v}{State : Type σ}{Obs : Type o}
+variable {EctxItem : Type i}
+
+class EvContextItem
+    (Expr : Type e)
+    (EctxItem : outParam (Type i)) where
+  fillItem : EctxItem → Expr → Expr
+  fillItem_inj {K} : Function.Injective (fillItem K)
+export EvContextItem (fillItem)
+
+attribute [simp] EvContextItem.fillItem_inj
+
+open BaseStep in
+class EctxItemLanguage
+    (Expr     : Type e)
+    (EctxItem : outParam <| Type i)
+    (State    : outParam <| Type σ)
+    (Obs      : outParam <| Type o)
+    (Val      : outParam <| Type v)
+  extends
+    ToVal Expr Val,
+    EvContextItem Expr EctxItem,
+    BaseStep Expr State Obs where
+
+  fillItem_val (e : Expr) (K : EctxItem) :
+    (toVal (fillItem K e)).isSome →
+    (toVal e).isSome
+
+  fillItem_no_val_inj (Ki₁ Ki₂ : EctxItem) :
+    toVal e₁ = none → toVal e₂ = none →
+    fillItem Ki₁ e₁ = fillItem Ki₂ e₂ →
+    Ki₁ = Ki₂
+
+  val_stuck : ∀ {e} {σ : State} {obs e' σ' eₜ},
+    (e, σ) -<obs>->ᵇ (e', σ', eₜ) → toVal e = none
+
+  -- base_ctx_step_val
+  base_ctx_step_val : ∀ {e} {σ : State} {obs e' σ' eₜ},
+    (fillItem Ki e, σ) -<obs>->ᵇ (e', σ', eₜ) →
+    (toVal e).isSome
+
+
+
+namespace EctxItemLanguage
+
+variable [Λ : EctxItemLanguage Expr EctxItem State Obs Val]
+
+abbrev Ectx [EvContext Expr EctxItem] := List EctxItem
+
+instance [EctxItemLanguage Expr EctxItem State Obs Val]:  EvContext Expr (List EctxItem) where
+  comp x y := y ++ x
+  empty := []
+  fill K e := K.foldl (fun x y => fillItem y x) e
+  fill_empty (e : Expr) := List.foldl_nil
+  fill_comp K₁ K₂ (e : Expr) := Eq.symm List.foldl_append
+  fill_inj {K} x y := by
+    induction K generalizing x y with
+    | nil => simp only [List.foldl_nil, imp_self]
+    | cons hd tl IH =>
+      simp at IH ⊢
+      intro sh
+      replace sh := IH _ _ sh
+      simpa only [EvContextItem.fillItem_inj, Function.Injective.eq_iff] using sh
+
+export EvContext (fill)
+
+@[rocq_alias fill_app]
+theorem fill_append (K1 K2 : List EctxItem) (e : Expr) :
+    fill (K1 ++ K2) e = fill K2 (fill K1 e) := by
+  dsimp [fill]
+  grind
+
+@[elab_as_elim] -- TODO: Properly more this from mathlib
+def reverseRec {motive : List α → Sort _} (nil : motive [])
+    (append_singleton : ∀ (l : List α) (a : α), motive l → motive (l ++ [a])) : ∀ l, motive l
+  | [] => nil
+  | x :: xs => by
+    have := List.eq_nil_or_concat (x :: xs)
+    cases this
+    case inl h => simp at h
+    case inr h =>
+      obtain ⟨init, l, h⟩ := h
+      rw [h]
+      have := reverseRec nil append_singleton init
+      have := append_singleton init l this
+      simpa
+termination_by l => l.length
+decreasing_by
+  simp at h
+  calc init.length
+    _ < (init ++ [l]).length := by grind
+    _ = (x :: xs).length := by grind
+
+theorem fill_val K (e : Expr) :
+    (toVal (fill K e)).isSome = true → (toVal e).isSome = true := by
+  induction K generalizing e with
+  | nil =>
+    dsimp [fill]
+    grind only
+  | cons init last IH =>
+    simp only [fill, List.foldl_cons] at IH ⊢
+    grind [fill, fillItem_val]
+
+theorem fill_not_val K (e : Expr) :
+     (toVal e) = none → (toVal (fill K e)) = none := by
+  grind [fill_val, Option.isSome_iff_ne_none]
+
+instance : EctxLanguage Expr (List EctxItem) State Obs Val where
+  fill_val K e := fill_val K e
+  step_by_val := by
+    intros K K' e₁ e₁' σ₁ obs e₂ σ₂ eₜ hfill hred hstep
+    induction K using reverseRec generalizing K' e₁ e₂ with
+    | nil =>
+      simp only [comp, List.append_nil, exists_eq']
+    | append_singleton Ks Ki IH =>
+      simp [comp]
+      simp [fill] at hfill
+      cases K' using reverseRec
+      · simp at hfill
+        subst hfill
+        replace hstep := base_ctx_step_val hstep |> fill_val _ _
+        grind
+      case append_singleton Ks' Ki' trash =>
+      simp at *
+      have heq : Ki = Ki' := by
+        apply Λ.fillItem_no_val_inj Ki Ki' _ _ hfill
+        · apply fill_not_val
+          assumption
+        · apply fill_not_val
+          apply val_stuck
+          assumption
+      subst heq
+      simp [Function.Injective.eq_iff] at hfill
+      simp [fill] at IH
+      obtain ⟨K'', rfl⟩ := IH hfill hred hstep
+      exists K''
+      simp [comp]
+  val_stuck {e σ obs e' σ' eₜ} := val_stuck
+  base_ctx_step_val {K e σ₁ obs e₂ σ₂ eₜ} := by
+    cases K using reverseRec
+    case nil =>
+      simp [empty]
+    case append_singleton init last IH =>
+      intro bstep
+      left
+      simp [fill_append] at *
+      apply fill_val
+      apply base_ctx_step_val
+      assumption
+
+theorem fill_no_val K (e : Expr) :
+    toVal e = none →
+    toVal (fill K e) = none := by
+  grind [fill_val]
+
+theorem subredexesAreValues (e : Expr) :
+    (∀ Ki e', e = fillItem Ki e' → (toVal e').isSome) →
+    EctxLanguage.subredexesAreValues e := by
+  rintro hsub K e' rfl
+  cases K using reverseRec
+  case nil => simp [empty]
+  case append_singleton init last IH =>
+    simp [empty, Option.ne_none_iff_exists]
+    suffices isSome : (toVal e').isSome from by
+      grind [Option.isSome_iff_exists]
+    apply fill_val
+    apply hsub
+    simp [fill]
+    rfl
+
+end EctxItemLanguage
